Clean up, getting things to compile

coq/LLVMGen/Correctness.v
@@ -115,7 +115,7 @@ Set Implicit Arguments.
 Set Strict Implicit.
 
 Import MDSHCOLOnFloat64.
-Import IO INT M Global Local.
+Import D IO INT M Global Local.
 Import TopLevelEnv.
 Import ListNotations.
 Import MonadNotation.
@@ -158,7 +158,7 @@ NOTEYZ: An alternative would be to translate everything that remains into failur
 
   (* We therefore have the following resulting denotation functions. *)
   (* On the Vellvm side, for [mcfg]: *)
-  Definition semantics_llvm_mcfg p : itree E_mcfg _ := translate_E_vellvm_mcfg (model_to_L3 helix_intrinsics p).
+  Definition semantics_llvm_mcfg p : itree E_mcfg _ := translate_E_vellvm_mcfg (model_to_L3 DTYPE_Void "Main" main_args helix_intrinsics p).
   (* Which get lifted to [toplevel_entity] as usual: *)
   Definition semantics_llvm (prog: list (toplevel_entity typ (list (LLVMAst.block typ)))) :=
     lift_sem_to_mcfg semantics_llvm_mcfg prog.
@@ -550,10 +550,22 @@ Ltac eutt_hide_right :=
     |- eutt _ _ ?t => remember t
   end.
 
-Ltac hide_string :=
+Ltac hide_string_goal :=
   match goal with
   | |- context [String ?x ?y] => remember (String x y)
   end.
+
+Ltac hide_string_hyp H :=
+  match type of H with
+  | context [String ?x ?y] => remember (String x y)
+  end.
+
+Ltac hide_strings :=
+  repeat (
+      match goal with
+      | h: context [String ?x ?y] |- _ => remember (String x y)
+      | |- context [String ?x ?y] => remember (String x y)
+      end).
 
 (* end tactics *)
 
@@ -652,7 +664,99 @@ Section InterpMem.
 
 End InterpMem.
 
-Section NEXP.
+
+  Ltac unfolderH H :=
+    unfold ErrorWithState.option2errS, translate_E_helix_cfg, lift_Serr in H.
+
+  Ltac unfolder_vellvm := unfold Traversal.Endo_id.
+    (* unfold lookup_E_to_exp_E,exp_E_to_instr_E. *)
+
+  Ltac unfolder_helix :=
+    unfold ErrorWithState.option2errS, translate_E_helix_cfg, lift_Serr, translate_E_vellvm_cfg.
+
+  (**
+     Better solution (?): use
+     `Argument myconstant /.`
+     to force `cbn` to unfold `myconstant`
+   *)
+  Ltac unfolder := unfolder_helix; unfolder_vellvm.
+
+  Tactic Notation "cbn*" := (repeat (cbn; unfolder)).
+
+  (** **
+      TODO YZ : This needs to leave other hypotheses that H untouched
+   *)
+  Ltac simp_comp H :=
+    cbn in H; unfolderH H;
+    cbn in H; repeat (inv_sum || break_and || break_match_hyp).
+
+  Lemma subevent_subevent : forall {E F} `{E -< F} {X} (e : E X),
+      @subevent F F _ X (@subevent E F _ X e) ≡ subevent X e.
+  Proof.
+    reflexivity.
+  Qed.
+
+  (* We associate [bind]s to the right and dismiss leftmost [Ret]s *)
+  Ltac norm_monad t :=
+    match t with
+    | context[ITree.bind ?t' _] =>
+      match t' with
+      | ITree.bind _ _ => rewrite bind_bind; idtac "bind_bind"
+      | Ret _ => rewrite bind_ret_l; idtac "bind_ret"
+      end
+    end.
+
+  (* We push [translate]s and [interp]s inside of binds, run them through [Ret]s *)
+  Ltac norm_interp t :=
+    match t with
+    | context[translate _ (ITree.bind ?t' _)] => rewrite translate_bind; idtac "trans_bind"
+    | context[interp _ (ITree.bind ?t' _)] => rewrite interp_bind; idtac "interp_bind"
+    | context[translate _ (Ret _)] => rewrite translate_ret; idtac "trans_ret"
+    | context[interp _ (Ret _)] => rewrite interp_ret; idtac "interp_ret"
+    | context[translate _ (trigger ?e)] => rewrite (translate_trigger _ e); idtac "trans_trigger"
+    | context[interp _ (trigger _)] => rewrite interp_trigger; idtac "intepr_trigger"
+    end.
+
+  (* We extend [norm_interp] with locally defined interpreters on the helix side *)
+  Ltac norm_local_helix t :=
+    match t with
+    | context[interp_Mem (ITree.bind ?t' _)] => rewrite interp_Mem_bind; idtac "mem_bind"
+    | context[interp_Mem (Ret _)] => rewrite interp_Mem_ret; idtac "mem_ret"
+    end.
+
+  (* We extend [norm_interp] with locally defined interpreters on the vellvm side *)
+  Ltac norm_local_vellvm t :=
+    match t with
+    | context[interp_cfg_to_L3 _ (ITree.bind ?t' _)] => rewrite interp_cfg_to_L3_bind; idtac "cfg_bind"
+    | context[interp_cfg_to_L3 _ (Ret _)] => rewrite interp_cfg_to_L3_ret; idtac "cfg_ret"
+    | context[interp_cfg_to_L3 _ (trigger (GlobalRead _))] => rewrite interp_cfg_to_L3_GR; idtac "cfg_GR"
+    | context[interp_cfg_to_L3 _ (trigger (LocalRead _))] => rewrite interp_cfg_to_L3_LR; idtac "cfg_LR"
+    | context[lookup_E_to_exp_E (subevent _ _)] => (rewrite lookup_E_to_exp_E_Global || rewrite lookup_E_to_exp_E_Local); try rewrite subevent_subevent; idtac "luexp"
+    | context[exp_E_to_instr_E (subevent _ _)] => (rewrite exp_E_to_instr_E_Global || rewrite exp_E_to_instr_E_Local); try rewrite subevent_subevent; idtac "expinstr"
+    end.
+
+  (**
+     QUESTION YZ: the outer repeat does not do effect. Why and how to fix?
+   *)
+  Ltac norm_h :=
+    match goal with
+      |- eutt _ ?t _ =>
+      repeat (
+          repeat (norm_monad t); 
+          repeat (norm_interp t);
+          repeat (norm_local_helix t))
+    end.
+
+  Ltac norm_v :=
+    match goal with
+      |- eutt _ _ ?t =>
+      repeat (
+          repeat (norm_monad t); 
+          repeat (norm_interp t);
+          repeat (norm_local_vellvm t))
+    end.
+
+Section NExpr.
 
   (**
      We prove in this section the correctness of the compilation of numerical expressions, i.e. [NExpr].
@@ -769,99 +873,74 @@ vars s1 = σ?
   context_lookup "NVar not found" σ v ≡ inr (DSHnatVal n) ->
   Maps.lookup id l ≡ Some (UVALUE_I64 n).
 
-  Ltac unfolderH H :=
-    unfold ErrorWithState.option2errS, translate_E_helix_cfg, lift_Serr in H.
-
-  Ltac unfolder_vellvm := unfold Traversal.Endo_id.
-    (* unfold lookup_E_to_exp_E,exp_E_to_instr_E. *)
-
-  Ltac unfolder_helix :=
-    unfold ErrorWithState.option2errS, translate_E_helix_cfg, lift_Serr, translate_E_vellvm_cfg.
-
-  (**
-     Better solution (?): use
-     `Argument myconstant /.`
-     to force `cbn` to unfold `myconstant`
-   *)
-  Ltac unfolder := unfolder_helix; unfolder_vellvm.
-
-  Tactic Notation "cbn*" := (repeat (cbn; unfolder)).
-
-  Ltac simp_comp H :=
-    cbn in H; unfolderH H;
-    cbn in H; repeat (inv_sum || break_and || break_match_hyp).
-
-  Lemma subevent_subevent : forall {E F} `{E -< F} {X} (e : E X),
-      @subevent F F _ X (@subevent E F _ X e) ≡ subevent X e.
-  Proof.
-    reflexivity.
-  Qed.
-
-  (* We associate [bind]s to the right and dismiss leftmost [Ret]s *)
-  Ltac norm_monad t :=
-    match t with
-    | context[ITree.bind ?t' _] =>
-      match t' with
-      | ITree.bind _ _ => rewrite bind_bind; idtac "bind_bind"
-      | Ret _ => rewrite bind_ret_l; idtac "bind_ret"
-      end
-    end.
-
-  (* We push [translate]s and [interp]s inside of binds, run them through [Ret]s *)
-  Ltac norm_interp t :=
-    match t with
-    | context[translate _ (ITree.bind ?t' _)] => rewrite translate_bind; idtac "trans_bind"
-    | context[interp _ (ITree.bind ?t' _)] => rewrite interp_bind; idtac "interp_bind"
-    | context[translate _ (Ret _)] => rewrite translate_ret; idtac "trans_ret"
-    | context[interp _ (Ret _)] => rewrite interp_ret; idtac "interp_ret"
-    | context[translate _ (trigger ?e)] => rewrite (translate_trigger _ e); idtac "trans_trigger"
-    | context[interp _ (trigger _)] => rewrite interp_trigger; idtac "intepr_trigger"
-    end.
-
-  (* We extend [norm_interp] with locally defined interpreters on the helix side *)
-  Ltac norm_local_helix t :=
-    match t with
-    | context[interp_Mem (ITree.bind ?t' _)] => rewrite interp_Mem_bind; idtac "mem_bind"
-    | context[interp_Mem (Ret _)] => rewrite interp_Mem_ret; idtac "mem_ret"
-    end.
-
-  (* We extend [norm_interp] with locally defined interpreters on the vellvm side *)
-  Ltac norm_local_vellvm t :=
-    match t with
-    | context[interp_cfg_to_L3 _ (ITree.bind ?t' _)] => rewrite interp_cfg_to_L3_bind; idtac "cfg_bind"
-    | context[interp_cfg_to_L3 _ (Ret _)] => rewrite interp_cfg_to_L3_ret; idtac "cfg_ret"
-    | context[interp_cfg_to_L3 _ (trigger (GlobalRead _))] => rewrite interp_cfg_to_L3_GR; idtac "cfg_GR"
-    | context[interp_cfg_to_L3 _ (trigger (LocalRead _))] => rewrite interp_cfg_to_L3_LR; idtac "cfg_LR"
-    | context[lookup_E_to_exp_E (subevent _ _)] => (rewrite lookup_E_to_exp_E_Global || rewrite lookup_E_to_exp_E_Local); try rewrite subevent_subevent; idtac "luexp"
-    | context[exp_E_to_instr_E (subevent _ _)] => (rewrite exp_E_to_instr_E_Global || rewrite exp_E_to_instr_E_Local); try rewrite subevent_subevent; idtac "expinstr"
-    end.
-
-  (**
-     QUESTION YZ: the outer repeat does not do effect. Why and how to fix?
-   *)
-  Ltac norm_h :=
-    match goal with
-      |- eutt _ ?t _ =>
-      repeat (
-          repeat (norm_monad t); 
-          repeat (norm_interp t);
-          repeat (norm_local_helix t))
-    end.
-
-  Ltac norm_v :=
-    match goal with
-      |- eutt _ _ ?t =>
-      repeat (
-          repeat (norm_monad t); 
-          repeat (norm_interp t);
-          repeat (norm_local_vellvm t))
-    end.
-
   (**
      QUESTION YZ: Works okay (though slow), except for [ret/Ret], a cbn or an unfold needs to be sneaked in the right place
+
+     TODO YZ : add that the returned IRState is also WF
    *)
 
-  (* TODOYZ: name consistency Nexp/NExpr/Nexpr/NExp *) 
+  Set Nested Proofs Allowed.
+
+  Lemma WFevalNexp_succeed:
+    forall nexp s s' σ x,
+      WF_IRState σ s ->
+      genNExpr nexp s ≡ inr (s',x) ->
+      WF_IRState σ s'.
+  Proof.
+    induction nexp; intros * WF GEN; simp_comp GEN; auto.
+    all: eapply IHnexp1 in Heqs0; eapply IHnexp2 in Heqs1; eauto.
+  Qed.
+
+  Lemma WFevalNexp_no_fail:
+    forall nexp s σ x msg,
+      WF_IRState σ s ->
+      genNExpr nexp s ≡ inr x ->
+      evalNexp σ nexp ≡ inl msg -> 
+      False.
+  Proof.
+    induction nexp; cbn; intros * WF COMP EVAL;
+      try now (simp_comp COMP; cbn in *; try inv_sum).
+    - unfold context_lookup, trywith in *.
+      cbn in COMP; unfolderH COMP; cbn in COMP.
+      simp_comp COMP; cbn in *; try inv_sum;
+        edestruct WF as (? & ? & ?); eauto.
+      all:try match goal with
+              | [h : ?x ≡ _ , h' : ?x ≡ _ |- _] => rewrite h in h'; inv h'
+              end.
+      all: match goal with
+           | h: getIRType _ ≡ _ |- _ => inv h
+           end.
+    - simp_comp COMP; cbn in *; try inv_sum.
+      eapply IHnexp1; eauto.
+      eapply IHnexp2; [eapply WFevalNexp_succeed | ..]; eauto. 
+    - simp_comp COMP; cbn in *; try inv_sum.
+      eapply IHnexp1; eauto.
+      eapply IHnexp2; [eapply WFevalNexp_succeed | ..]; eauto. 
+    - simp_comp COMP; cbn in *; try inv_sum.
+      eapply IHnexp1; eauto.
+      eapply IHnexp2; [eapply WFevalNexp_succeed | ..]; eauto. 
+    - simp_comp COMP; cbn in *; try inv_sum.
+      eapply IHnexp1; eauto.
+      eapply IHnexp2; [eapply WFevalNexp_succeed | ..]; eauto. 
+    - simp_comp COMP; cbn in *; try inv_sum.
+      eapply IHnexp1; eauto.
+      eapply IHnexp2; [eapply WFevalNexp_succeed | ..]; eauto. 
+  Qed.
+
+  (* TODO use Vellvm/Tactics *)
+  Ltac ret_bind_l_left v :=
+    match goal with
+      |- eutt _ ?t _ =>
+      rewrite <- (bind_ret_l v (fun _ => t))
+    end.
+
+  (* TODO MOVE *)
+  Lemma convert_typ_app : ∀ (a b : code typ) env, (convert_typ env (a ++ b) ≡ convert_typ env a ++ convert_typ env b)%list.
+  Proof.
+    induction a as [| [] a IH]; cbn; intros; auto.
+    rewrite IH; reflexivity.
+  Qed.
+
   Lemma genNExpr_correct :
     forall (* Compiler bits *) (s1 s2: IRState)
       (* Helix  bits *)   (nexp: NExpr) (σ: evalContext) (memH: memoryH)
@@ -869,20 +948,22 @@ vars s1 = σ?
       genNExpr nexp s1 ≡ inr (s2, (exp, c)) -> (* Compilation succeeds *)
       WF_IRState σ s1 ->                       (* Well-formed IRState *)
       R σ memH (memV, (l, g)) ->
-      eutt (lift_R_memory_cfg R σ ⩕ lift_R_result_cfg R' σ)
-           (translate_E_helix_cfg  
-              (interp_Mem (denoteNexp σ nexp)
-                          memH))
-           (translate_E_vellvm_cfg
-              ((interp_cfg_to_L3 helix_intrinsics
-                                 (D.denote_code (convert_typ [] c) ;; translate exp_E_to_instr_E (D.denote_exp None (convert_typ [] exp))))
-                 g l memV)).
+      (* (WF_IRState σ s2 /\ *)
+       eutt (lift_R_memory_cfg R σ ⩕ lift_R_result_cfg R' σ)
+            (translate_E_helix_cfg  
+               (interp_Mem (denoteNexp σ nexp)
+                           memH))
+            (translate_E_vellvm_cfg
+               ((interp_cfg_to_L3 helix_intrinsics
+                                  (D.denote_code (convert_typ [] c) ;; translate exp_E_to_instr_E (D.denote_exp (Some (DTYPE_I 64%Z)) (convert_typ [] exp))))
+                  g l memV)).
   Proof.
-    induction nexp; intros * COMPILE WFIR PRE;
+    intros s1 s2 nexp; revert s1 s2; induction nexp; intros * COMPILE WFIR PRE;
       assert (FOO: (s2,(exp,c)) ≡ (s2,(exp,c))) by reflexivity. (* TODOYZ: stupid hack to quickly check what case we are in. To remove *)
     - (* Variable case *)
 
       (* Reducing the compilation *)
+      (* simp_comp COMPILE; (split; [auto |]). *)
       simp_comp COMPILE.
 
       + (* The variable maps to an integer in the IRState *)
@@ -926,1418 +1007,448 @@ vars s1 = σ?
 
     - (* Constant *)
 
-      simp_comp COMPILE.
+      simp_comp COMPILE(* ; split; auto *).
       unfold denoteNexp; cbn*.
       repeat norm_h.
       repeat norm_v.
-      (** ** TODO
-          The compiler appears to generate invalid code:
-          (raise "denote_exp given untyped EXP_Integer")
-       *)
-
-          (* Reducing the denotation *)
-          unfold denoteNexp; cbn*.
-          repeat norm_v.
-          break_inner_match_goal.
-          { (* Variable not in context, [context_lookup] fails *)
-            abs_by WF_IRState_lookup_cannot_fail.
-          }
-          break_inner_match_goal.
-          ++ exfalso.
-             clear FOO.
-             repeat norm_h.
-             destruct i0.
-             { (* Global *)
-               cbn*.
-               repeat norm_v.
-               cbn; repeat norm_v.
-               2: eapply R_GLU; eauto.
-               cbn*; repeat norm_v.
-               repeat norm_h.
-
-               rewrite interp_cfg_to_L3_LM.
-
-
-
-
-               rewrite translate_trigger. lookup_E_to_exp_E_Global.
-
-               2: eapply R_GLU; eauto.
-               (** TODO: Define specialized version on eutt for external use *)
-               apply eqit_Ret.
-               split; [apply PRE | reflexivity].
-             }
-             { (* Local *)
-               cbn*.
-               repeat norm_v.
-               2: eapply R_LLU; eauto.
-               cbn; repeat norm_v.
-               apply eqit_Ret.
-               split; [apply PRE | reflexivity].
-             }
-          ++
-            (** TODO YZ : get this automatically discharged by [abs_by] *)
-            exfalso. eapply WF_IRState_lookup_int in WFIR; eauto.
-            destruct WFIR as [? WFIR]; rewrite Heqs in WFIR; inv WFIR.
-          ++
-            exfalso. eapply WF_IRState_lookup_int in WFIR; eauto.
-            destruct WFIR as [? WFIR]; rewrite Heqs in WFIR; inv WFIR.
-
-
-
-          
-
-
-          unfold translate_E_helix_cfg; cbn.
-          unfold denoteNexp, lift_Serr; cbn.
-          match goal with
-            |- context[context_lookup ?s ?x ?y] => destruct (context_lookup s x y) as [? | []] eqn:?EQ
-          end.
-          exfalso; admit.
-          unfold translate_E_helix_cfg; cbn; rewrite interp_Mem_ret, translate_ret.
-          admit.
-          exfalso; admit.
-          exfalso; admit.
-
-    - (* Constant *)
-      simp_comp COMPILE.
-
-      unfold translate_E_helix_cfg; cbn; rewrite interp_Mem_ret, translate_ret.
-      (* Ret (memH, t) *)
-      admit.
-
+      apply eqit_Ret.
+      split; [apply PRE |].
+      rewrite repr_intval; reflexivity.
+      
     - (* NDiv *)
 
       simp_comp COMPILE.
 
-      unfold denoteNexp; cbn.
-      break_match_goal.
-      exfalso; admit.
-      break_match_goal.
-      exfalso; admit.
-      unfold translate_E_helix_cfg; cbn; rewrite interp_Mem_ret, translate_ret.
-      admit.
+      generalize Heqs; intros WFI; eapply WFevalNexp_succeed in WFI; eauto.
 
-    - 
-      simp_comp COMPILE.
-      admit.
+      eutt_hide_right.
+      unfold denoteNexp in *; cbn*.
 
-    - (* NPlus *)
-
-      simp_comp COMPILE.
-      admit.
-
-    - admit.
-
-  (* Relations for expressions *)
-  (* top might be able to just be Some (DTYPE_I 64) *)
-  (* NOTEYZ: I am completely confused by this definition. *)
-  Definition nexp_relation
-             (env : list (ident * typ))
-             (e : exp typ)
-             (n : Int64.int)
-             (r : (memory * (local_env * (global_env * ())))): Prop :=
-    let '(mem_llvm, (ρ, (g, _))) := r in
-    eutt (fun n '(_, (_, (_, uv))) => int64_concrete_uvalue_rel n uv)
-         (ret n)
-         (interp_cfg_to_L3 helix_intrinsics (translate exp_E_to_instr_E (D.denote_exp (Some (DTYPE_I 64)) (TransformTypes.fmap_exp _ _ (TypeUtil.normalize_type_dtyp env) e))) g ρ mem_llvm).
-
-  (**
-     Division case. Division by zero is ruled out by assuming that no failure can happen.
-     TODOYZ: Do we:
-      - rule out failure from the source program (usual assumption, sensible). If so, how to we express it?
-      - prove preservation of failure. Unusual, stronger, require a change in our current non-interpretation of errors.
-   *)
-  (* TODO: Need something about denoteNexp not failing *)
-  Lemma denote_nexp_div :
-    forall (σ : evalContext) (nexp1 nexp2 : NExpr),
-      eutt Logic.eq (denoteNexp σ (NDiv nexp1 nexp2))
-           (ITree.bind (denoteNexp σ nexp1)
-                       (fun (n1 : Int64.int) => ITree.bind (denoteNexp σ nexp2)
-                                                        (fun (n2 : Int64.int) => denoteNexp σ (NDiv (NConst n1) (NConst n2))))).
-  Proof.
-  Admitted.
-
-
-  (* TODOCB: do I need something relating IRstate and evalContext? *)
-  (* TODOYZ: Cleanup the normalization of types layer.
-             Should we have a typeclass to have a uniform way to normalize the sub-pieces of code?
-   *)
-  (* TODOYZ: Apparently, this might be dead code.
-             There's also [denote_exp_nexp], [interp_denoteNexp_genNExpr] and [interp_cfg_to_L3_denote_exp]
-   *)
-
-  Lemma denoteNexp_genNExpr :
-    forall (* Helix bits  *) (nexp : NExpr) (σ : evalContext) (st st' : IRState) mem_helix
-      (* Vellvm bits *) (nexp_r : exp typ) (nexp_code : code typ) (env : list (ident * typ))  g ρ mem_llvm,
-      (* TODOCB: Do I need mem_helix?
-         YZ: I suspect it depends on whether you run the interpreter [interp_Mem] or not here
-       *)
-      memory_invariant σ mem_helix (mem_llvm, (ρ, g)) ->
-      genNExpr nexp st  ≡ inr (st', (nexp_r, nexp_code)) ->
-      eutt (nexp_relation env nexp_r)
-           (translate inr_ (denoteNexp σ nexp))
-           (translate inl_ (interp_cfg_to_L3 helix_intrinsics
-                             (D.denote_code (map
-                                               (λ '(id, i),
-                                                (id, TransformTypes.fmap_instr typ dtyp (TypeUtil.normalize_type_dtyp env) i))
-                                               nexp_code)) g ρ mem_llvm)).
-  Proof.
-    (*
-    induction nexp; intros σ st st' mem_helix nexp_r nexp_code env g ρ mem_llvm Hmem H.
-    - (* NVar *)
-      cbn in H.
-      repeat break_match_hyp; subst; inversion H; simpl.
-      + cbn in Heqs.
-        subst.
-        rewrite interp_cfg_to_L3_ret.
-        destruct (nth_error (vars st) v) eqn:Hnth; inversion Heqs; subst.
-        unfold denoteNexp. cbn.
-        unfold context_lookup.
-        destruct (nth_error σ v) eqn:Hnthsigma.
-        cbn. destruct d.
-        cbn.
-        do 2 rewrite translate_ret.
-        apply eqit_Ret.
-        cbn.
-        * destruct i0; cbn.
-          rewrite bind_trigger.
-          repeat rewrite translate_vis.
-          cbn.
-
-          unfold interp_cfg_to_L3.
-          unfold INT.interp_intrinsics.
-          rewrite interp_vis.
-          cbn.
-          rewrite interp_global_bind.
-          unfold INT.F_trigger.
-          unfold interp_global at 2.
-          setoid_rewrite interp_state_trigger.
-          rewrite bind_bind.
-          cbn.
-          break_match.
-          2: admit. (* exception *)
-          rewrite bind_ret_l.
-          rewrite bind_tau.
-          rewrite tau_eutt.
-          rewrite bind_ret_l.
-          rewrite tau_eutt.
-          rewrite interp_translate.
-          cbn.
-          rewrite translate_ret.
-          rewrite interp_ret.
-          rewrite interp_global_ret.
-          rewrite interp_local_ret.
-          rewrite M.interp_memory_ret.
-
-          apply eqit_Ret.
-
-          unfold int64_concrete_uvalue_rel.
-          rewrite uvalue_to_dvalue_of_dvalue_to_uvalue.
-          unfold int64_dvalue_rel.
-          inversion Hmem.
-          apply ListUtil.length_0 in H0; subst.
-          rewrite ListNth.nth_error_nil in Hnthsigma. inversion Hnthsigma.
-          destruct H0.
-          pose proof (H0 v (DSHnatVal n) Hnthsigma).
-          cbn in H1.
-          destruct H1 as (? & ? & ? & ? & ? & ? & ?).
-          subst.
-          destruct H1. admit.
-          cbn.
-
-          admit.
-          admit.
-        * admit.
-        * admit.
-        * admit.
-      +
-      (* exception *) admit.
-
-      (*
-        destruct t.
-        destruct (Z.eq_dec sz 64).
-        inversion H. reflexivity.
-        inversion H.
-        destruct t.
-        *
-      + inversion H.
-       *)
-    - (* NConst *)
-      cbn in H; inversion H; cbn.
-      rewrite interp_cfg_to_L3_ret.
-      repeat rewrite translate_ret.
-      apply eqit_Ret.
-      cbn.
-      rewrite translate_ret.
-      rewrite interp_cfg_to_L3_ret.
-      apply eqit_Ret.
-      cbn.
-      rewrite DynamicValues.Int64.unsigned_repr.
-      apply Z.eq_refl.
-      pose proof (DynamicValues.Int64.intrange t).
-      unfold DynamicValues.Int64.max_unsigned.
-      omega.
-    - cbn in H.
-      repeat break_match_hyp; inversion H.
-
-      repeat rewrite map_app.
-      repeat setoid_rewrite denote_code_app.
-
-      rewrite denote_nexp_div.
-      pose proof IHnexp1 σ _ _ mem_helix _ _ env g ρ mem_llvm Hmem Heqs.
-      rewrite interp_cfg_to_L3_bind.
-      repeat setoid_rewrite translate_bind.
-      eapply eutt_clo_bind; eauto.
-
-      intros u1 u2 H4.
-      repeat break_match.
-      rewrite interp_cfg_to_L3_bind; rewrite translate_bind.
-      eapply eutt_clo_bind; eauto.
-      (* eapply H0. *)
-
-      (* intros u0 u3 H5. *)
-      (* repeat break_match. *)
-
-      (* (* We executed code that generated the values for the *)
-      (* expressions for the binary operations... Now we need to denote *)
-      (* the expressions themselves. *) *)
-      (* (* simplify left side to ret *) *)
-      (* cbn. *)
-
-      (* repeat rewrite translate_bind.       *)
-      (* repeat rewrite interp_cfg_to_L3_bind. *)
-      (* repeat rewrite bind_bind. *)
-
-      (* genNExpr nexp1 st ≡ inr (i, (e, c)) *)
-      (* I need something relating `denote_exp e` and `denoteNexp nexp1`... *)
-     *)
-  Admitted.
-
-  Lemma denote_exp_nexp:
-    forall nexp st i e c mem_llvm σ g ρ env,
-      genNExpr nexp st ≡ inr (i, (e, c)) ->
-      (* TODO: factor out this relation *)
-      eutt (fun n '(m, (l, (g, uv))) => int64_concrete_uvalue_rel n uv)
-           (translate inr_ (denoteNexp σ nexp))
-           (translate inl_ (interp_cfg_to_L3 helix_intrinsics (translate exp_E_to_instr_E (D.denote_exp (Some (DTYPE_I 64)) (TransformTypes.fmap_exp _ _ (TypeUtil.normalize_type_dtyp env) e))) g ρ mem_llvm)).
-  Proof.
-    induction nexp; intros st i e c mem_llvm σ g ρ env H.
-    - cbn in H; repeat break_match_hyp; try solve [inversion H].
-      + (* Int case *)
-        cbn.
-        unfold denoteNexp. cbn.
-        break_match.
-        * cbn.
-          (* exception *) admit.
-        * break_match.
-          -- inversion H. cbn.
-             (* Need something linking id to global_env / local_env *)
-             destruct i1.
-             ++ cbn. rewrite bind_trigger.
-                repeat rewrite translate_vis.
-                admit.
-             ++ admit.
-          -- cbn. (* exception *) admit.
-          -- cbn. (* exception *) admit.
-      + (* Pointer case *)
-        admit.
-    - cbn in H; repeat break_match_hyp; inversion H; cbn.
-      admit.
-  Admitted.
-
-  (* TODO: awful AWFUL name. Need to figure out which of these we need *)
-  Definition nexp_relation_mem (σ : evalContext) (helix_res : MDSHCOLOnFloat64.memory * Int64.int) (llvm_res : TopLevelEnv.memory * (local_env * (global_env * ()))) : Prop
-    :=
-      let '(mem_helix, n) := helix_res in
-      let '(mem_llvm, (ρ, (g, _))) := llvm_res in
-      memory_invariant σ mem_helix (mem_llvm, (ρ, g)).
-
-  Lemma interp_denoteNexp_genNExpr :
-    forall (nexp : NExpr) (st st' : IRState) (nexp_r : exp typ) (nexp_code : code typ) (env : list (ident * typ)) (σ : evalContext) g ρ mem_llvm memory,
-      genNExpr nexp st  ≡ inr (st', (nexp_r, nexp_code)) ->
-      eutt (nexp_relation_mem σ)
-           (translate inr_ (interp_state (case_ Mem_handler MDSHCOLOnFloat64.pure_state) (denoteNexp σ nexp) memory))
-           (translate inl_ (interp_cfg_to_L3 helix_intrinsics
-                                             (D.denote_code (map
-                                                               (λ '(id, i),
-                                                                (id, TransformTypes.fmap_instr typ dtyp (TypeUtil.normalize_type_dtyp env) i))
-                                                               nexp_code)) g ρ mem_llvm)).
-  Proof.
-  Admitted.
-
-  Lemma interp_cfg_to_L3_denote_exp :
-    forall nexp s s' ll_exp ll_code n m l g env σ,
-      genNExpr nexp s ≡ inr (s', (ll_exp, ll_code)) ->
-      denoteNexp σ nexp ≈ Ret n ->
-      (interp_cfg_to_L3 helix_intrinsics
-                        (translate exp_E_to_instr_E
-                                   (D.denote_exp (Some (DTYPE_I 64))
-                                                 (TransformTypes.fmap_exp typ dtyp (TypeUtil.normalize_type_dtyp env) ll_exp))) g l m) ≈ Ret (m, (l, (g, UVALUE_I64 n))).
-  Proof.
-    induction nexp;
-      intros s s' ll_exp ll_code n m l g env σ H H0;
-      cbn in H; inversion H.
-    - (* NVar *)
-      admit.
-    (* Exceptions due to lookup and type mismatches! *)
-    - (* NConst *)
-      cbn. rewrite repr_intval.
-      rewrite translate_ret, interp_cfg_to_L3_ret.
-      apply eqit_inv_ret in H0; subst; auto.
-      reflexivity.
-    - (* NDiv *)
-      rewrite denote_nexp_div in H0.
-      cbn in *.
-  Admitted.
-
-  Lemma eval_denoteNexp :
-    forall σ nexp val,
-      evalNexp σ nexp ≡ inr val ->
-      denoteNexp σ nexp ≅ Ret val.
-  Proof.
-    intros σ nexp val H.
-    unfold denoteNexp. rewrite H.
-    reflexivity.
-  Qed.
-
-  (* Unprovable, this should come from some well typedness assumption *)
-  Lemma nvar_is_i64 :
-    forall {v s s' s'' ll_exp ll_code str i t},
-      genNExpr (NVar v) s ≡ inr (s', (ll_exp, ll_code)) ->
-      getStateVar str v s ≡ inr (s'', (i, t)) ->
-      t ≡ TYPE_I 64%Z.
-  Proof.
-  Admitted.
-
-  (* TODO: This is WRONG
-
-      Each instruction evaluated in the code that nexp produces can
-      add a local variable.
-   *)
-  Lemma denote_code_of_nexp :
-    forall nexp s s' ll_exp ll_code env mem_llvm g ρ,
-      genNExpr nexp s ≡ inr (s', (ll_exp, ll_code)) ->
-      exists ρ',
-        interp_cfg_to_L3 helix_intrinsics
-                         (D.denote_code
-                            (map (λ '(id, i), (id, TransformTypes.fmap_instr typ dtyp (TypeUtil.normalize_type_dtyp env) i))
-                                 ll_code)) g ρ mem_llvm ≈ Ret (mem_llvm, (ρ', (g, ()))).
-  Proof.
-    induction nexp;
-      intros s s' ll_exp ll_code env mem_llvm g ρ H;
-      remember H as Hgen eqn:Heqgen; clear Heqgen;
-        inversion H; subst; cbn.
-    -  cbn in H.
-       break_match_hyp; inversion H1.
-       destruct p, p.
-       pose proof (nvar_is_i64 Hgen Heqs0); subst.
-       break_match_hyp; try contradiction.
-       exists ρ.
-       inversion H1; subst.
-       cbn.
-       rewrite interp_cfg_to_L3_ret.
-       reflexivity.
-    - exists ρ. rewrite interp_cfg_to_L3_ret.
-      reflexivity.
-    - exists ρ. (* TODO: This will need to change *)
-
-        break_match_hyp.
-        inversion H1.
-        repeat break_match_hyp.
-        inversion H1.
-        inversion H1.
-        cbn in *.
-        do 2 rewrite map_app.
-        do 2 setoid_rewrite denote_code_app.
-        setoid_rewrite bind_bind.
-
-        rewrite interp_cfg_to_L3_bind.
-        pose proof IHnexp1 s i e c env mem_llvm g ρ Heqs0 as [ρ' Hnexp1].
-        rewrite Hnexp1.
-        rewrite bind_ret_l.
-
-        rewrite interp_cfg_to_L3_bind.
-        pose proof IHnexp2 i i0 e0 c0 env mem_llvm g ρ' Heqs1 as [ρ'' Hnexp2].
-        rewrite Hnexp2.
-        rewrite bind_ret_l.
-
-        cbn.
-        repeat setoid_rewrite translate_bind.
-        rewrite bind_bind.
-
-        rewrite interp_cfg_to_L3_bind.
-
-  Admitted.
-
-  (* TODO: I think I might want to know that ρ comes from denoting ll_code, actually *)
-  Lemma denote_exp_of_nexp :
-    forall nexp ll_exp ll_code s s' env g ρ mem_llvm mem_helix σ i,
-      memory_invariant σ mem_helix (mem_llvm, (ρ, g)) ->
-      genNExpr nexp s ≡ inr (s', (ll_exp, ll_code)) ->
-      evalNexp σ nexp ≡ inr i ->
-      (interp_cfg_to_L3 helix_intrinsics
-                        (translate exp_E_to_instr_E
-                                   (D.denote_exp (Some (TypeUtil.normalize_type_dtyp env Utils.IntType))
-                                                 (TransformTypes.fmap_exp typ dtyp (TypeUtil.normalize_type_dtyp env) ll_exp))) g ρ mem_llvm) ≈ Ret (mem_llvm, (ρ, (g, UVALUE_I64 i))).
-  Proof.
-    setoid_rewrite normalize_IntType.
-    induction nexp;
-      intros ll_exp ll_code s s' env g ρ mem_llvm mem_helix σ i Hmem H H0;
-      inversion H; inversion H0; subst; cbn.
-    - repeat break_match_hyp; inversion H3; inversion H2;
-        cbn.
-      destruct i1; cbn.
-      rewrite bind_trigger.
-      repeat setoid_rewrite translate_vis.
-      repeat setoid_rewrite translate_ret.
-
-
-      unfold interp_cfg_to_L3.
-      {
-        Set Nested Proofs Allowed.
-
+      break_inner_match_goal; [| break_inner_match_goal].
+      + clear - Heqs Heqs1 WFIR; abs_by WFevalNexp_no_fail. 
+      + clear - Heqs0 WFI Heqs2; abs_by WFevalNexp_no_fail. 
+      + repeat norm_h.
         
-      setoid_rewrite interp_intrinsics_vis; cbn.
-      unfold INT.F_trigger.
-      rewrite bind_trigger.
-      setoid_rewrite interp_global_vis; cbn.
+        (* TODO YZ: gets some super specialize tactics that do not require to provide variables *)
+        specialize (IHnexp1 _ _ _ _ _ _ _ _ _ Heqs WFIR PRE).
+        ret_bind_l_left i2.
+        subst.
+        eutt_hide_left.
+        cbn*.
+        repeat norm_v.
+        unfold convert_typ.
 
-      unfold memory_invariant in Hmem.
-      unfold context_lookup in Heqs0. destruct (nth_error σ v) eqn:Hlookup; inversion Heqs0.
-      destruct Hmem as [Hmem | Hmem].
-      { (* Case where sigma is nil *)
-        assert (σ ≡ []) by (apply ListUtil.length_0; auto).
-        subst; cbn in Hlookup; rewrite ListNth.nth_error_nil in Hlookup.
-        inversion Hlookup.
-      }
+        rewrite convert_typ_app. rewrite denote_code_app.
+        repeat norm_v.
+        subst.
 
-      destruct Hmem as [iota Hmem].
-      (* TODO: need to be able to relate
+        (* unfold translate_E_vellvm_cfg in *. *)
+        (* cbn in IHnexp1. *)
+        (* rewrite interp_cfg_to_L3_bind in IHnexp1. *)
+        (* rewrite translate_bind in IHnexp1. *)
+        (* eapply eutt_clo_bind. *)
+        admit.       
 
-            alist_find AstLib.eq_dec_raw_id id g
+  Admitted.
 
-            and ι somehow.
+End NExpr.
+
+Section MExpr.
+
+  (** ** Compilation of MExpr TODO
+  *)
+  Lemma genMExpr_correct : forall R R',
+    forall (* Compiler bits *) (s1 s2: IRState)
+      (* Helix  bits *)   (mexp: MExpr) (σ: evalContext) (memH: memoryH)
+      (* Vellvm bits *)   (exp: exp typ) (c: code typ) (g : global_env) (l : local_env) (memV : memoryV) (τ: typ),
+      genMExpr mexp s1 ≡ inr (s2, (exp, c, τ)) -> (* Compilation succeeds *)
+      WF_IRState σ s1 ->                            (* Well-formed IRState *)
+      R σ memH (memV, (l, g)) ->
+      (* (WF_IRState σ s2 /\ *)
+       eutt R' 
+            (translate_E_helix_cfg  
+               (interp_Mem (denoteMexp σ mexp)
+                           memH))
+            (translate_E_vellvm_cfg
+               ((interp_cfg_to_L3 helix_intrinsics
+                                  (D.denote_code (convert_typ [] c) ;; translate exp_E_to_instr_E (D.denote_exp (Some (DTYPE_I 64%Z)) (convert_typ [] exp))))
+                  g l memV)).
+  Proof.
+  Admitted.
+
+End MExpr.
+
+Section AExpr.
+
+  (** ** Compilation of MExpr TODO
+  *)
+  Lemma genAExpr_correct : forall R R',
+    forall (* Compiler bits *) (s1 s2: IRState)
+      (* Helix  bits *)   (aexp: AExpr) (σ: evalContext) (memH: memoryH)
+      (* Vellvm bits *)   (exp: exp typ) (c: code typ) (g : global_env) (l : local_env) (memV : memoryV) (τ: typ),
+      genAExpr aexp s1 ≡ inr (s2, (exp, c)) -> (* Compilation succeeds *)
+      WF_IRState σ s1 ->                            (* Well-formed IRState *)
+      R σ memH (memV, (l, g)) ->
+      (* (WF_IRState σ s2 /\ *)
+       eutt R' 
+            (translate_E_helix_cfg  
+               (interp_Mem (denoteAexp σ aexp)
+                           memH))
+            (translate_E_vellvm_cfg
+               ((interp_cfg_to_L3 helix_intrinsics
+                                  (D.denote_code (convert_typ [] c) ;; translate exp_E_to_instr_E (D.denote_exp (Some (DTYPE_I 64%Z)) (convert_typ [] exp))))
+                  g l memV)).
+  Proof.
+  Admitted.
+
+End AExpr.
+
+Section MemCopy.
+  (** ** Compilation of MemCopy TODO
+      Unclear how to state this at the moment.
+      What is on the Helix side? What do the arguments correspond to?
+   *)
+
+  Lemma genMemCopy_correct : 
+    forall (* Compiler bits *) (s1 s2: IRState)
+      (* Helix  bits *)   (σ: evalContext) 
+      (* Vellvm bits *)   (o: Int64.int) (x y: ident) (nextblock bid: block_id) (bks : list (LLVMAst.block typ)), 
+      genMemCopy o x y nextblock s1 ≡ inr (s2, (bid, bks)) -> (* Compilation succeeds *)
+      WF_IRState σ s1 ->                                      (* Well-formed IRState *)
+      False.
+      (* eutt R' 
+            (translate_E_helix_cfg  
+               (interp_Mem (denoteAexp σ aexp)
+                           memH))
+            (translate_E_vellvm_cfg
+               ((interp_cfg_to_L3 helix_intrinsics
+                                  (D.denote_code (convert_typ [] c) ;; translate exp_E_to_instr_E (D.denote_exp (Some (DTYPE_I 64%Z)) (convert_typ [] exp))))
+                  g l memV)).
        *)
-
-            Lemma gen_var_irstate_rel :
-              forall v s s' ll_exp ll_code mem_helix σ mem_llvm ρ g i id sz,
-                genNExpr (NVar v) s ≡ inr (s', (ll_exp, ll_code)) ->
-                memory_invariant σ mem_helix (mem_llvm, (ρ, g)) ->
-                evalNexp σ (NVar v) ≡ inr i ->
-                getStateVar "NVar out of range" v s ≡ inr (s', (ID_Global id, TYPE_I sz)) ->
-                alist_find AstLib.eq_dec_raw_id id g ≡ Some (DVALUE_I64 i).
-            Proof.
-              intros v s s' ll_exp ll_code mem_helix σ mem_llvm ρ g i id sz H H0 H1 H2.
-              cbn in H1. break_match_hyp; inversion H1.
-              break_match_hyp; inversion H1; subst.
-              unfold context_lookup in *.
-              destruct (nth_error σ v) eqn:Hlookup.
-              2: { inversion Heqs0. }
-              cbn in H2.
-              destruct (nth_error (vars s) v) eqn:Hlookupst.
-              2: { inversion H2. }
-              cbn in H2.
-              inversion H2. subst.
-              inversion Heqs0.
-              subst.
-              unfold memory_invariant in H0.
-              rename H0 into Hmem.
-              destruct Hmem as [Hmem | Hmem].
-              { (* Case where sigma is nil *)
-                assert (σ ≡ []) by (apply ListUtil.length_0; auto).
-                subst; cbn in Hlookup; rewrite ListNth.nth_error_nil in Hlookup.
-                inversion Hlookup.
-              }
-
-              destruct Hmem as (Hinj & ?).
-              specialize (H0 _ _ Hlookup).
-
-              destruct H0 as [ptr_llvm [[[Hlocal Hnotglobal] | [Hnotlocal Hglobal]]
-                                 [bk_llvm [Hlogicalblock [v_llvm [Hlookup_block Hmatches]]]]]]; subst.
-
-              admit. (* locals *)
-
-              cbn.
-
-              cbn in *; subst.
-
-            Qed.
-
-
-
-End NEXP.
-
-
-(* CHECKPOINTYZ: Continue the dive from there Tomorrow *)
-
-(* Lemma LLVMGen_correct: forall i o globals op name newstate pll (σ: evalContext), *)
-(*   LLVMGen i o globals false op name newState ≡ inr pll -> *)
-(*   eutt (bisim_final σ) *)
-(*        (translate (@subevent _ E_mcfg _) *)
-(*                   (interp_Mem (denoteDSHOperator σ op) memory_empty)) *)
-(*        (semantics_llvm pll). *)
-
-(* Top-level compiler correctness lemma  *)
-(* Theorem compiler_correct: *)
-(*   forall (p:FSHCOLProgram) *)
-(*     (data:list binary64) *)
-(*     (pll: toplevel_entities typ (list (LLVMAst.block typ))), *)
-(*     compile_w_main p data ≡ inr pll -> *)
-(*     eutt (bisim_final []) (semantics_FSHCOL p data) (semantics_llvm pll). *)
-(* Proof. *)
-(*   intros p data pll H. *)
-(*   unfold compile_w_main, compile in H. *)
-(*   destruct p as [i o name globals op]. *)
-(*   destruct (initIRGlobals data globals) as [? | [data' ginit]] eqn:EQGlob; [inv H |]. *)
-(*   simpl in H. *)
-(*   destruct (ErrorWithState.evalErrS (LLVMGen i o globals false op name) newState) eqn: EQEVALERR; [inv H | inv H]. *)
-(*   unfold semantics_llvm. *)
-(*   unfold semantics_llvm_mcfg. *)
-(*   unfold lift_sem_to_mcfg. *)
-(*   match goal with *)
-(*     |- context[match ?p with | _ => _ end] => destruct p eqn:EQ *)
-(*   end. { *)
-(*     unfold ErrorWithState.evalErrS in EQEVALERR. *)
-(*     destruct (LLVMGen i o globals false op name newState) eqn:EQGEN; inv EQEVALERR. *)
-
-(*   (* This no longer follows from [compiler_correct_aux]. It will *)
-(*      at pen-ultimate step when the [main] does [return] on a memory *)
-(*      block. *)
-
-(*        eapply eqit_mon. *)
-(*        3:apply bisim_full_final_subrelation. *)
-(*        3:eapply compiler_correct_aux. *)
-(*        tauto. *)
-(*        tauto. *)
-(*        tauto. *)
-(*    *) *)
-(* Admitted. *)
-
-
-Definition blah {T} (defs : IS.intrinsic_definitions) (m : memory) (g : global_env) (l : local_env) (e : instr_E T) :=
-  M.interp_memory (interp_local (interp_global (INT.interp_intrinsics_h defs e) g) l) m.
-(*
-  (State.interp_state
-         (case_ (M.E_trigger (F:=PickE +' UBE +' DebugE +' FailureE))
-            (case_ M.handle_intrinsic (case_ M.handle_memory (M.F_trigger (F:=PickE +' UBE +' DebugE +' FailureE)))))
-         (State.interp_state (interp_local_h (G:=MemoryE +' PickE +' UBE +' DebugE +' FailureE))
-            (State.interp_state (interp_global_h (G:=LLVMEnvE +' MemoryE +' PickE +' UBE +' DebugE +' FailureE))
-               (INT.interp_intrinsics_h defs e) g) l) m).
-*)
-
-Import Coq.Strings.String Strings.Ascii.
-Open Scope string_scope.
-Open Scope char_scope.
-
-  (* TODO: Prove and move to itrees *)
-  Lemma interp_state_interp :
-    ∀ (E F G : Type -> Type) (R : Type) (ST : Type) (st : ST)
-      (f : ∀ T : Type, E T → itree F T) (g : forall T : Type, F T -> Monads.stateT ST (itree G) T) (t : itree E R),
-      interp_state g (interp f t) st ≅ interp_state (fun (T : Type) (e : E T) => interp g (f T e)) t st.
   Proof.
   Admitted.
 
-  (* TODO: Move to itrees? *)
-  (* Check interp_interp. *)
-  (* Lemma interp_state_interp_state : *)
-  (*   forall (E G H : Type -> Type) (R STF STG T: Type) *)
-  (*     (f : ∀ T : Type, E T → Monads.stateT STF (itree G) T) *)
-  (*     (g : forall T : Type, G T -> Monads.stateT STG (itree H) T) *)
-  (*     (sf : STF) (sg : STG) *)
-  (*     (t : itree E R) t', *)
-  (*     interp_state g (interp_state f t sf) sg ≅ t'. *)
-  (* Proof. *)
-  (*   intros. *)
-  (*   unfold interp_state. *)
-  (*   Check interp_interp. *)
+End MemCopy.
 
-  (*   Check interp g (fun T e => f T e sf) sg. *)
-  (*   setoid_rewrite interp_interp. *)
-  (*   Set Nested Proofs Allowed. *)
-  (*   assert (itree H (STG * (STF * R))). *)
-  (*   refine (interp_state _ _ _). *)
-  (*   refine (@interp_state G _ STG _ _ _ _ _). *)
+Section FSHAssign.
+  (** ** Compilation of FSHAssign TODO
+      Unclear how to state this at the moment
+      What is on the Helix side? What do the arguments correspond to?
+   *)
 
-  (*   (fun (T : Type) (e : E T) => _) t). *)
-  (* Qed. *)
-
-
-(*
-    for an opeartor, in initialized state
-    TODO: We could probably fix [env] to be [nil]
- *)
-
-  Lemma DSHAssign_singleton :
-    forall (nextblock : block_id) (src dst : MemVarRef) (st st' : IRState) (bid_in : block_id)
-      (bks : list (LLVMAst.block typ)),
-      genIR (DSHAssign src dst) nextblock st ≡ inr (st', (bid_in, bks)) ->
-      exists b,
-        genIR (DSHAssign src dst) nextblock st ≡ inr (st', (bid_in, [b]))
-        /\ snd (blk_term b) ≡ TERM_Br_1 nextblock
-        /\ blk_id b ≡ bid_in /\ bks ≡ [b].
+  Lemma genFSHAssign_correct : 
+    forall (* Compiler bits *) (s1 s2: IRState)
+      (* Helix  bits *)   (σ: evalContext) 
+      (* Vellvm bits *)   (i o: Int64.int) (x y: ident) (src dst: NExpr) (nextblock bid: block_id) (bks : list (LLVMAst.block typ)), 
+      genFSHAssign i o x y src dst nextblock s1 ≡ inr (s2, (bid, bks)) -> (* Compilation succeeds *)
+      WF_IRState σ s1 ->                                      (* Well-formed IRState *)
+      False.
+      (* eutt R' 
+            (translate_E_helix_cfg  
+               (interp_Mem (denoteAexp σ aexp)
+                           memH))
+            (translate_E_vellvm_cfg
+               ((interp_cfg_to_L3 helix_intrinsics
+                                  (D.denote_code (convert_typ [] c) ;; translate exp_E_to_instr_E (D.denote_exp (Some (DTYPE_I 64%Z)) (convert_typ [] exp))))
+                  g l memV)).
+       *)
   Proof.
-    intros nextblock src dst st st' bid_in bks HCompile.
-    simpl in HCompile. destruct src, dst.
-    simpl in HCompile.
-    repeat break_match_hyp; try inl_inr.
-    inv Heqs; inv HCompile.
-    unfold genFSHAssign in Heqs2.
-    cbn in Heqs2.
   Admitted.
 
-  Lemma genIR_DSHAssign_to_genFSHAssign :
-    forall src dst nextblock st st' b,
-      genIR (DSHAssign src dst) nextblock st ≡ inr (st', (blk_id b, [b])) ->
-      exists psrc nsrc pdst ndst b_orig comments i i0 i1 i2 i3 n n0,
-        src ≡ (psrc, nsrc) /\
-        dst ≡ (pdst, ndst) /\
-        [b] ≡ add_comment [b_orig] comments /\
-        resolve_PVar psrc st ≡ inr (i, (i0, n)) /\
-        resolve_PVar pdst i  ≡ inr (i1, (i2, n0)) /\
-        genFSHAssign n n0 i0 i2 nsrc ndst nextblock i1 ≡ inr (i3, (blk_id b, [b_orig])).
+End FSHAssign.
+
+Section WhileLoop.
+  (** ** Compilation of loops TODO
+      Unclear how to state this at the moment
+      What is on the Helix side? What do the arguments correspond to?
+   *)
+
+  Lemma genWhileLoop_correct : 
+    forall (* Compiler bits *) (s1 s2: IRState)
+      (* Helix  bits *) (σ: evalContext) 
+      (* Vellvm bits *) (prefix: string) (from to: exp typ) (loopvar: raw_id) (loopcontblock: block_id)
+                        (body_entry: block_id) (body_blocks: list (LLVMAst.block typ)) (init_code: (code typ))
+                        (nextblock: block_id) (bid: block_id) (bks : list (LLVMAst.block typ)), 
+      genWhileLoop prefix from to loopvar loopcontblock body_entry body_blocks init_code nextblock s1 ≡ inr (s2, (bid, bks)) -> (* Compilation succeeds *)
+      WF_IRState σ s1 ->                                      (* Well-formed IRState *)
+      False.
+      (* eutt R' 
+            (translate_E_helix_cfg  
+               (interp_Mem (denoteAexp σ aexp)
+                           memH))
+            (translate_E_vellvm_cfg
+               ((interp_cfg_to_L3 helix_intrinsics
+                                  (D.denote_code (convert_typ [] c) ;; translate exp_E_to_instr_E (D.denote_exp (Some (DTYPE_I 64%Z)) (convert_typ [] exp))))
+                  g l memV)).
+       *)
   Proof.
-    intros src dst nextblock st st' b H.
-    destruct src as (psrc, nsrc). exists psrc. exists nsrc.
-    destruct dst as (pdst, ndst). exists pdst. exists ndst.
+  Admitted.
 
-    inv H.
-    destruct (resolve_PVar psrc st) eqn:Hr. inversion H1.
-    destruct p. destruct p.
-    destruct (resolve_PVar pdst i) eqn:Hr1. inversion H1.
-    destruct p. destruct p.
-    destruct (genFSHAssign i1 i4 i0 i3 nsrc ndst nextblock i2) eqn:Hassign. inversion H1.
-    destruct p. destruct s.
-    match goal with
-    | H: context[add_comment _ ?ss] |- _ => remember ss
-    end.
+End WhileLoop.
 
-    inversion H1.
-    apply add_comment_singleton in H3. destruct H3 as (b_orig & Hl).
-    exists b_orig. exists l0.
-    exists i. exists i0. exists i2. exists i3. exists i5. exists i1. exists i4.
-    subst; intuition.
-  Qed.
+Section IMapBody.
+  (** ** Compilation of IMapBody TODO
+   *)
 
-(*   Lemma compile_NExpr_correct : *)
-(*     forall (nexp : NExpr) (e : exp typ) (c : code typ) (σ : evalContext) env (mem : MDSHCOLOnFloat64.memory) s s' mem_llvm ρ g, *)
-(*       genNExpr nexp s ≡ inr (s', (e, c)) -> *)
-(*       eutt _ *)
-(*            (translate inr_ (interp_Mem (denoteNexp σ nexp) mem)) *)
-(*            (translate inl_ (interp_cfg_to_L3 helix_intrinsics *)
-(*                                              (D.denote_code ((map (λ '(id, i), (id, TransformTypes.fmap_instr typ dtyp (TypeUtil.normalize_type_dtyp env) i)) *)
-(*                                                                   c))) *)
-(*                                              g ρ mem_llvm)). *)
-
-(* (map (λ '(id, i), (id, TransformTypes.fmap_instr typ dtyp (TypeUtil.normalize_type_dtyp env) i)) *)
-(*                    src_nexpcode) *)
-
-
-  (* Probably need to know something about σ and mem_llvm,
-     like memory_invariant... *)
-
-  (* Print LLVMGEnvE. *)
-  Lemma interp_cfg_to_L3_globalread :
-    forall g1 l0 m4 id d,
-      alist_find AstLib.eq_dec_raw_id id g1 ≡ Some d ->
-      (interp_cfg_to_L3 helix_intrinsics (trigger (GlobalRead id))
-                        g1 l0 m4) ≈ (Ret (m4, (l0, (g1, d)))).
+  Lemma genIMapBody_correct : 
+    forall (* Compiler bits *) (s1 s2: IRState)
+      (* Helix  bits *) (σ: evalContext) (f: AExpr)
+      (* Vellvm bits *) (n: Int64.int) (x y: ident) (loopvar: raw_id) (nextblock: block_id) (bid: block_id) (bks: list (LLVMAst.block typ)),
+      genIMapBody n x y f loopvar nextblock s1 ≡ inr (s2, (bid, bks)) -> (* Compilation succeeds *)
+      WF_IRState σ s1 ->                                      (* Well-formed IRState *)
+      False.
+      (* eutt R' 
+            (translate_E_helix_cfg  
+               (interp_Mem (denoteAexp σ aexp)
+                           memH))
+            (translate_E_vellvm_cfg
+               ((interp_cfg_to_L3 helix_intrinsics
+                                  (D.denote_code (convert_typ [] c) ;; translate exp_E_to_instr_E (D.denote_exp (Some (DTYPE_I 64%Z)) (convert_typ [] exp))))
+                  g l memV)).
+       *)
   Proof.
-    intros.
-    unfold interp_cfg_to_L3, M.interp_memory, interp_local, interp_global, INT.interp_intrinsics.
-    setoid_rewrite interp_vis.
-    repeat setoid_rewrite interp_state_bind.
-    cbn. unfold INT.F_trigger.
+  Admitted.
 
-    setoid_rewrite interp_state_trigger.
-    repeat setoid_rewrite interp_state_bind.
-    rewrite bind_bind.
+End IMapBody.
 
-    cbn. rewrite H.
-    repeat setoid_rewrite interp_state_ret.
-    rewrite bind_ret_l.
-    repeat rewrite interp_state_tau.
-    rewrite bind_tau.
-    repeat rewrite interp_state_ret.
-    rewrite bind_ret_l.
-    cbn.
-    repeat rewrite interp_state_tau.
-    rewrite interp_ret.
-    repeat rewrite interp_state_ret.
+Section BinOpBody.
+  (** ** Compilation of IMapBody TODO
+   *)
 
-    rewrite tau_eutt.
-    rewrite tau_eutt.
-    reflexivity.
-  Qed.
-
-  Lemma denotePexp_eutt_ret :
-    forall (σ : evalContext) (v : var_id) a size,
-      nth_error σ v ≡ Some (DSHPtrVal a size) ->
-      denotePexp σ (PVar v) ≈ Ret a.
+  Lemma genBinOpBody_correct : 
+    forall (* Compiler bits *) (s1 s2: IRState)
+      (* Helix  bits *) (σ: evalContext) (f: AExpr)
+      (* Vellvm bits *) (n: nat) (x y: ident) (loopvar: raw_id) (nextblock: block_id) (bid: block_id) (bks: list (LLVMAst.block typ)),
+      genBinOpBody n x y f loopvar nextblock s1 ≡ inr (s2, (bid, bks)) -> (* Compilation succeeds *)
+      WF_IRState σ s1 ->                                      (* Well-formed IRState *)
+      False.
+      (* eutt R' 
+            (translate_E_helix_cfg  
+               (interp_Mem (denoteAexp σ aexp)
+                           memH))
+            (translate_E_vellvm_cfg
+               ((interp_cfg_to_L3 helix_intrinsics
+                                  (D.denote_code (convert_typ [] c) ;; translate exp_E_to_instr_E (D.denote_exp (Some (DTYPE_I 64%Z)) (convert_typ [] exp))))
+                  g l memV)).
+       *)
   Proof.
-    intros σ v a size H.
-    unfold denotePexp; cbn.
-    rewrite H.
-    reflexivity.
-  Qed.
+  Admitted.
+
+End BinOpBody.
+
+Section MemMap2Body.
+  (** ** Compilation of IMapBody TODO
+   *)
+
+  Lemma genMemMap2Body_correct : 
+    forall (* Compiler bits *) (s1 s2: IRState)
+      (* Helix  bits *) (σ: evalContext) (f: AExpr)
+      (* Vellvm bits *) (n: nat) (x x0 y: ident) (loopvar: raw_id) (nextblock: block_id) (bid: block_id) (bks: list (LLVMAst.block typ)),
+      genMemMap2Body n x x0 y f loopvar nextblock s1 ≡ inr (s2, (bid, bks)) -> (* Compilation succeeds *)
+      WF_IRState σ s1 ->                                      (* Well-formed IRState *)
+      False.
+      (* eutt R' 
+            (translate_E_helix_cfg  
+               (interp_Mem (denoteAexp σ aexp)
+                           memH))
+            (translate_E_vellvm_cfg
+               ((interp_cfg_to_L3 helix_intrinsics
+                                  (D.denote_code (convert_typ [] c) ;; translate exp_E_to_instr_E (D.denote_exp (Some (DTYPE_I 64%Z)) (convert_typ [] exp))))
+                  g l memV)).
+       *)
+  Proof.
+  Admitted.
+
+End MemMap2Body.
+
+Section MemInit.
+  (** ** Compilation of IMapBody TODO
+      Hmm this one even refuses to get admitted!
+   *)
+
+(*
+  Lemma genMemInit_correct : 
+    forall (* Compiler bits *) (s1 s2: IRState)
+      (* Helix  bits *) (σ: evalContext) (initial: binary64)
+      (* Vellvm bits *) (size: Int64.int) (y: ident) (nextblock: block_id) (bid: block_id) (bks: list (LLVMAst.block typ)),
+      genMemInit size y initial nextblock s1 ≡ inr (s2, (bid, bks)) -> (* Compilation succeeds *)
+      WF_IRState σ s1 ->                                      (* Well-formed IRState *)
+      False.
+      (* eutt R' 
+            (translate_E_helix_cfg  
+               (interp_Mem (denoteAexp σ aexp)
+                           memH))
+            (translate_E_vellvm_cfg
+               ((interp_cfg_to_L3 helix_intrinsics
+                                  (D.denote_code (convert_typ [] c) ;; translate exp_E_to_instr_E (D.denote_exp (Some (DTYPE_I 64%Z)) (convert_typ [] exp))))
+                  g l memV)).
+       *)
+  Proof.
+  Admitted.
+  *)
+
+End MemInit.
+ 
+Section Power.
+  (** ** Compilation of IMapBody TODO
+   *)
+
+  Lemma genPower_correct : 
+    forall (* Compiler bits *) (s1 s2: IRState)
+      (* Helix  bits *) (σ: evalContext) (src dst: NExpr) (n: NExpr) (f: AExpr)
+      (* Vellvm bits *) (i o: Int64.int) (x y: ident) (initial: binary64) (nextblock: block_id) (bid: block_id) (bks: list (LLVMAst.block typ)),
+      genPower i o x y src dst n f initial nextblock s1 ≡ inr (s2, (bid, bks)) -> (* Compilation succeeds *)
+      WF_IRState σ s1 ->                                      (* Well-formed IRState *)
+      False.
+      (* eutt R' 
+            (translate_E_helix_cfg  
+               (interp_Mem (denoteAexp σ aexp)
+                           memH))
+            (translate_E_vellvm_cfg
+               ((interp_cfg_to_L3 helix_intrinsics
+                                  (D.denote_code (convert_typ [] c) ;; translate exp_E_to_instr_E (D.denote_exp (Some (DTYPE_I 64%Z)) (convert_typ [] exp))))
+                  g l memV)).
+       *)
+  Proof.
+  Admitted.
+
+End Power.
+
+Tactic Notation "cbn*" ident(H) := (repeat (cbn in H; unfolderH H)).
+
+(* TO MOVE *)
+Global Instance ConvertTyp_list {A} `{Traversal.Fmap A}: ConvertTyp (fun T => list (A T)) :=
+  fun env => Traversal.fmap (typ_to_dtyp env).
+
+Variant Box (T: Type): Type := box (t: T).
+(* Protects from "direct" pattern matching but not from context one *)
+Ltac protect H := apply box in H.
+Ltac hide_string_hyp' H :=
+  match type of H with
+  | context [String ?x ?y] =>
+    let msg := fresh "msg" in
+    let eqmsg := fresh "EQ_msg" in
+    remember (String x y) as msg eqn:eqmsg; protect eqmsg
+  end.
+
+Ltac hide_strings' :=
+  repeat (
+      match goal with
+      | h: Box _ |- _ => idtac
+      | h: context [String ?x ?y] |- _ =>
+        let msg := fresh "msg" in
+        let eqmsg := fresh "EQ_msg" in
+        remember (String x y) as msg eqn:eqmsg;
+        protect eqmsg
+      | |- context [String ?x ?y] =>
+        let msg := fresh "msg" in
+        let eqmsg := fresh "EQ_msg" in
+        remember (String x y) as msg eqn:eqmsg;
+        protect eqmsg
+      end).
+
+Ltac forget_strings :=
+  repeat (
+      match goal with
+      | h: context [String ?x ?y] |- _ =>
+        let msg := fresh "msg" in
+        generalize (String x y) as msg
+      | |- context [String ?x ?y] =>
+        let msg := fresh "msg" in
+        generalize (String x y) as msg
+      end).
 
 
-(* TODO: only handle cases where there are no exceptions? *)
-Lemma compile_FSHCOL_correct
-      (op: DSHOperator): forall (nextblock bid_in : block_id) (st st' : IRState) (bks : list (LLVMAst.block typ)) (σ : evalContext) (env : list (ident * typ)) (mem : MDSHCOLOnFloat64.memory) (g : global_env) (ρ : local_env) (mem_llvm : memory),
-  nextblock ≢ bid_in ->
-  bisim_partial σ (mem,tt) (mem_llvm, (ρ, (g, (inl bid_in)))) ->
-  genIR op nextblock st ≡ inr (st',(bid_in,bks)) ->
-  eutt (bisim_partial σ)
-       (translate inr_
-                  (interp_Mem (denoteDSHOperator σ op) mem))
-       (translate inl_
-                  (interp_cfg_to_L3 helix_intrinsics
-                                    (D.denote_bks (fmap (typ_to_dtyp env) bks) bid_in)
-                                    g ρ mem_llvm)).
-Proof.
-  induction op; intros; rename H1 into HCompile.
-  - inv HCompile.
-    eutt_hide_right; cbn.
-    unfold interp_Mem; simpl denoteDSHOperator.
-    rewrite interp_state_ret, translate_ret.
-    subst i. 
-    rewrite denote_bks_nil.
-    cbn. rewrite interp_cfg_to_L3_ret, translate_ret.
-    apply eqit_Ret; auto.
-  - (*
+Section GenIR.
+
+  (* YZ TODO : reducing denote_bks exposes iter. Should we simply make it opaque? *)
+  Opaque denote_bks.
+  Opaque resolve_PVar genFSHAssign.
+  
+  Lemma compile_FSHCOL_correct :
+    forall (** Compiler bits *) (s1 s2: IRState) 
+      (** Helix bits    *) (op: DSHOperator) (σ : evalContext) (memH : memoryH)
+      (** Vellvm bits   *) (nextblock bid_in : block_id) (bks : list (LLVMAst.block typ))
+      (env : list (ident * typ))  (g : global_env) (ρ : local_env) (memV : memoryV),
+      nextblock ≢ bid_in -> (* YZ: not sure about this yet *)
+      bisim_partial σ (memH,tt) (memV, (ρ, (g, (inl bid_in)))) ->
+      genIR op nextblock s1 ≡ inr (s2,(bid_in,bks)) ->
+      eutt (bisim_partial σ)
+           (translate_E_helix_cfg
+              (interp_Mem (denoteDSHOperator σ op) memH))
+           (translate_E_vellvm_cfg
+              (interp_cfg_to_L3 helix_intrinsics
+                                (D.denote_bks (convert_typ env bks) bid_in)
+                                g ρ memV)).
+  Proof.
+    intros s1 s2 op; revert s1 s2; induction op; intros * NEXT BISIM GEN.
+    - cbn in GEN.
+      hide_strings'.
+      simp_comp GEN.
+      eutt_hide_right; cbn*; repeat norm_h; subst.
+      cbn*; repeat norm_v.
+      (* YZ TODO : add denote_bks theory to the automation *)
+      rewrite denote_bks_nil.
+      cbn*; repeat norm_v.
+      apply eqit_Ret; auto.
+
+    - (*
       Assign case.
        Need some reasoning about
        - resolve_PVar
        - genFSHAssign
        - D.denote_bks over singletons
-     *)
-    apply DSHAssign_singleton in HCompile.
-    destruct HCompile as (b & HCompile & Hterm & Hbid & Hbksbk).
-    subst.
+       *)
+      destruct src,dst,p.
+      cbn* GEN.
+      hide_strings'.
+      simp_comp GEN.
 
-    (* Start by working on the left hand side *)
-
-
-
-    unfold normalize_types_blocks.
-    eutt_hide_left.
-    unfold fmap; simpl Fmap_list'.
-    (* Rewrite denote_bks to denote_block *)
-    rewrite denote_bks_singleton; eauto using normalize_types_block_term.
-
-    (* Work with denote_block *)
-    (* I need to know something about b... *)
-    pose proof genIR_DSHAssign_to_genFSHAssign src dst nextblock st HCompile as H1.
-    destruct H1 as (psrc & nsrc & pdst & ndst & b_orig & comments & ist & i0 & ist1 & i1 & ist2 & n & n0 & Hsrc & Hdst & Hb & Hr & Hr' & Hfsh).
-
-    cbn in Hb. inversion Hb.
-    cbn.
-
-    (* Now I need to know something about b_orig... *)
-    (* I know it's generated from genFSHassign, though... *)
-    cbn in Hfsh.
-
-    (* Checkpoint *)
-    inversion Hfsh.
-    destruct (genNExpr nsrc
-                       {|
-                         block_count := S (block_count ist1);
-                         local_count := S (S (S (local_count ist1)));
-                         void_count := S (S (void_count ist1));
-                         vars := vars ist1 |}) as [|(s', (src_nexpr, src_nexpcode))] eqn:Hnexp_src. inversion H3.
-    destruct (genNExpr ndst s') as [|(s'', (dst_nexpr, dst_nexpcode))] eqn:Hnexp_dst. inversion H3.
-    inversion H3.
-    cbn.
-    (*
-    match goal with
-    | |- context[D.denote_code (map _ (src_nexpcode ++ dst_nexpcode ++ ?x))] => remember x as assigncode
-    end.
-
-    (* start working on right side again *)
-    subst i. cbn.
-    subst src dst.
-
-    destruct psrc as [src_v] eqn:Hpsrc, pdst as [dst_v] eqn:Hpdst.
-
-    destruct (nth_error σ dst_v) as [d|] eqn:Hdst_v. 2: admit. (* Exception *)
-    destruct d as [n_dst | v_dst | a_dst size_dst]. admit. admit. (* should only be able to be pointer *)
-
-    destruct (nth_error σ src_v) as [d|] eqn:Hsrc_v. 2: admit. (* Exception *)
-    destruct d as [n_src | v_src | a_src size_src]. admit. admit. (* should only be able to be pointer *)
-
-    setoid_rewrite denotePexp_eutt_ret; eauto.
-
-    repeat rewrite bind_ret_l.
-    repeat setoid_rewrite bind_trigger.
-
-    (* Should be able to handle MemLU's in a lemma as well *)
-    destruct (memory_lookup_err "Error looking up 'x' in DSHAssign" mem a_src) eqn:Hmem_src.
-    admit. (* Exception *)
-
-    destruct (memory_lookup_err "Error looking up 'y' in DSHAssign" mem a_dst) eqn:Hmem_dst.
-    admit. (* Exception *)
-    cbn.
-
-    repeat (rewrite interp_Mem_MemLU; eauto).
-
-    destruct (evalNexp σ nsrc) as [|eval_src] eqn:Heval_src.
-    admit. (* Exception *)
-
-    destruct (evalNexp σ ndst) as [|eval_dst] eqn:Heval_dst.
-    admit. (* Exception *)
-
-    setoid_rewrite eval_denoteNexp; eauto.
-    repeat setoid_rewrite bind_ret_l.
-    cbn.
-
-    destruct (mem_lookup_err "Error looking up 'v' in DSHAssign" (MInt64asNT.to_nat eval_src) m) eqn:Hmemlookup.
-    admit. (* Exception *)
-    cbn.
-    rewrite bind_ret_l.
-
-    rewrite interp_Mem_MemSet.
-
-    (* Work on the right hand side again *)
-    (* Unfold denote_code and break it apart. *)
-    do 2 rewrite map_app.
-    do 2 setoid_rewrite denote_code_app.
-    do 2 setoid_rewrite bind_bind.
-
-    repeat setoid_rewrite interp_cfg_to_L3_bind.
-    repeat setoid_rewrite translate_bind.
-
-    (* Need to relate denoteNexp and denote_code of genNexpr *)
-    match goal with
-    | |- context[ ITree.bind ?x ?y ] => remember y as BLAH
-    end.
-
-    Set Nested Proofs Allowed.
-
-            Lemma irstate_rel (op: DSHOperator) :
-              forall (nextblock bid_in : block_id) (st st' : IRState) (bks : list (LLVMAst.block typ)) (σ : evalContext) (env : list (ident * typ)) (mem : MDSHCOLOnFloat64.memory) (g : global_env) (ρ : local_env) (mem_llvm : memory),
-                nextblock ≢ bid_in -> (* Do I need this? *)
-                bisim_partial σ (mem,tt) (mem_llvm, (ρ, (g, (inl bid_in)))) ->
-                genIR op nextblock st ≡ inr (st',(bid_in,bks)) ->
-
-
-            Lemma lookup_global:
-              forall σ mem_helix mem_llvm ρ g v i id s s' sz,
-                memory_invariant σ mem_helix (mem_llvm, (ρ, g)) ->
-                getStateVar "NVar out of range" v s ≡ inr (s', (ID_Global id, TYPE_I sz)) ->
-                evalNexp σ (NVar v) ≡ inr i ->
-                exists a, alist_find AstLib.eq_dec_raw_id id g ≡ Some (DVALUE_Addr a).
-            Proof.
-              intros σ mem_helix mem_llvm ρ g v i id s s' sz Hmem Hst Heval.
-              cbn in Heval.
-              unfold context_lookup in *.
-              destruct (nth_error σ v) eqn:Hlookup; cbn in Heval; try solve [inversion Heval].
-              unfold memory_invariant in Hmem.
-              destruct Hmem as [Hmem | Hmem].
-              { (* Case where sigma is nil *)
-                assert (σ ≡ []) by (apply ListUtil.length_0; auto).
-                subst; cbn in Hlookup; rewrite ListNth.nth_error_nil in Hlookup.
-                inversion Hlookup.
-              }
-
-              destruct Hmem as (Hinj & ?).
-              specialize (H _ _ Hlookup).
-
-              (* Determine that d = DSHnatVal i *)
-              destruct d eqn:Hd; cbn in Heval; inversion Heval as [Hni]; rewrite Hni in *.
-
-              destruct H as [ptr_llvm [[[Hlocal Hnotglobal] | [Hnotlocal Hglobal]]
-                                 [bk_llvm [Hlogicalblock [v_llvm [Hlookup_block Hmatches]]]]]]; subst.
-
-              (* Variable is in the local environment *)
-              admit.
-
-              (* Variable is in the global environment *)
-              exists ptr_llvm. unfold inj_f in Hglobal.
-              destruct Hinj.
-              cbn in Hglobal.
-
-              (* Need something relating id and v *)
-              destruct (inj_f0 v).
-
-              - (* d = DSHnatVal i *)
-                destruct H as
-                    [ptr_llvm [[[Hlocal Hnotglobal] | [Hnotlocal Hglobal]]
-                                 [bk_llvm [Hlogicalblock [v_llvm [Hlookup_block Hmatches]]]]]]; subst.
-                admit.
-
-                exists ptr_llvm.
-                unfold inj_f in Hglobal.
-                destruct Hinj.
-                destruct inj_f0.
-
-
-                unfold Hinj in
-
-                 destruct Hsearch.
-
-            Qed.
-            .
-              inversio
-
-
-            destruct (alist_find AstLib.eq_dec_raw_id id g) eqn:Hg.
-            Focus 2. admit. (* Exception *)
-
-            rewrite bind_ret_l.
-            repeat rewrite tau_eutt.
-            cbn.
-            rewrite interp_ret.
-            rewrite interp_global_ret.
-            cbn.
-
-            setoid_rewrite interp_local_ret.
-            unfold M.interp_memory.
-            rewrite interp_state_ret.
-
-            (* Need something relating g... memory_invariant ? *)
-
-            setoid_rewrite interp_memory_ret.
-            rewrite
-            inversion Heqs1; subst.
-            rewrite interp_cfg_to_L3_vis.
-            setoid_rewrite tau_eutt.
-            cbn.
-            setoid_rewrite translate_vis.
-            repeat rewrite translate_vis.
-            do 2 setoid_rewrite interp_cfg_to_L3_vis; cbn.
-            rewrite bind_bind.
-            setoid_rewrite interp_cfg_to_L3_vis.
-            rewrite bind_bind.
-            setoid_rewrite interp_cfg_to_L3_vis.
-            rewrite bind_bind.
-            setoid_rewrite interp_cfg_to_L3_vis.
-            rewrite bind_bind.
-            repeat setoid_rewrite translate_ret.
-            setoid_rewrite interp_intrinsics_vis.
-            cbn;
-            rewrite interp_cfg_to_L3_vis.
-          - rewrite translate_ret, interp_cfg_to_L3_ret, repr_intval.
-            reflexivity.
-          -
-        Qed.
-
-        cbn.
-        subst.
-        rewrite IHnexp1.
-
-        destruct (genNExpr nexp1 s) eqn:Hnexp1.
-        inversion H1.
-        destruct p, p.
-
-        destruct (genNExpr nexp1 s) eqn:Hnexp1.
-    Qed.
-
-
-
-      memory * (local_env * (global_env * ()))memory * (local_env * (global_env * ()))
-    Lemma interp_nex
-    subst assigncode.
-              cbn.
-
-              repeat setoid_rewrite translate_bind.
-              repeat setoid_rewrite interp_cfg_to_L3_bind.
-              repeat setoid_rewrite bind_bind.
-
-              destruct i0 eqn:Hi0.
-              ** (* Global id *)
-                repeat setoid_rewrite translate_bind.
-                rewrite interp_cfg_to_L3_bind.
-                repeat setoid_rewrite translate_vis.
-                repeat setoid_rewrite bind_bind.
-                repeat setoid_rewrite translate_ret.
-
-                destruct (alist_find AstLib.eq_dec_raw_id id g1) eqn:Hlookup.
-                Focus 2. admit. (* Exception *)
-
-                cbn.
-
-                match goal with
-                | |- context [ ITree.bind ?x ?y ] => remember y
-                end.
-
-                setoid_rewrite interp_cfg_to_L3_globalread; eauto.
-
-                rewrite translate_bind.
-                rewrite bind_bind.
-                repeat rewrite translate_ret.
-                rewrite bind_ret_l.
-                repeat rewrite translate_ret.
-                rewrite interp_cfg_to_L3_ret.
-                rewrite translate_ret.
-                rewrite bind_ret_l.
-
-                subst i3; cbn.
-
-                match goal with
-                | |- context [ ITree.bind ?x ?y ] => remember y
-                end.
-
-                repeat setoid_rewrite bind_bind.
-                setoid_rewrite translate_ret.
-                setoid_rewrite bind_ret_l.
-
-                rewrite interp_cfg_to_L3_bind.
-                rewrite translate_bind.
-                rewrite bind_bind.
-
-                rewrite normalize_IntType.
-                progress cbn.
-                rewrite translate_ret.
-                rewrite interp_cfg_to_L3_ret.
-                rewrite translate_ret, bind_ret_l.
-                cbn.
-
-                rewrite interp_cfg_to_L3_bind.
-                rewrite interp_cfg_to_L3_denote_exp; eauto.
-
-                (* This feels very stupid, surely this should all just evaluate? *)
-                rewrite translate_bind.
-                rewrite translate_ret.
-                rewrite bind_ret_l.
-                rewrite interp_cfg_to_L3_bind.
-                rewrite translate_bind.
-                rewrite interp_cfg_to_L3_ret.
-                rewrite translate_ret, bind_ret_l.
-                repeat rewrite interp_cfg_to_L3_bind.
-                rewrite interp_cfg_to_L3_ret.
-                rewrite bind_ret_l.
-                cbn.
-
-                rewrite uvalue_to_dvalue_of_dvalue_to_uvalue.
-                unfold ITree.map.
-                rewrite bind_trigger.
-                rewrite translate_vis.
-                cbn.
-                setoid_rewrite translate_ret.
-
-                subst i3.
-                cbn.
-
-                all: eauto.
-                Focus 2. apply Hnexp_src.
-                reflexivity.
-
-                setoid_rewrite bind_ret_l.
-                setoid_rewrite <- denote_exp_nexp.
-                apply eutt_clo_bind.
-
-                rewrite interp
-                rewrite bind_trigger.
-                rewrite translate_vis.
-                rewrite translate_vis.
-                setoid_rewrite translate_ret.
-                setoid_rewrite translate_ret.
-                cbn.
-                repeat setoid_rewrite translate_bind.
-                rewrite interp_cfg_to_L3_bind.
-                repeat setoid_rewrite translate_vis.
-                repeat setoid_rewrite bind_bind.
-                repeat setoid_rewrite translate_ret.
-
-                rewrite interp_cfg_to_L3_vis; cbn.
-                repeat setoid_rewrite bind_bind.
-                cbn.
-                rewrite translate_bind.
-                rewrite bind_bind.
-                cbn.
-
-                match goal with
-                | |- context[ITree.bind ?ma ?b] => remember b as blah
-                end.
-
-                unfold interp_cfg_to_L3; cbn.
-                unfold trigger.
-                rewrite interp_intrinsics_vis.
-                cbn.
-                setoid_rewrite tau_eutt.
-                setoid_rewrite interp_ret.
-                setoid_rewrite bind_ret_r.
-                unfold interp_global.
-                cbn.
-                unfold M.interp_memory.
-                unfold interp_local.
-                cbn.
-
-                unfold INT.F_trigger.
-                setoid_rewrite interp_state_trigger.
-                cbn.
-                destruct (alist_find AstLib.eq_dec_raw_id id g1) eqn:Hg1.
-                Focus 2.
-                (* exception *) admit.
-                rewrite bind_ret_l.
-                repeat rewrite interp_state_tau.
-                rewrite tau_eutt.
-                repeat rewrite interp_state_ret.
-                rewrite translate_ret.
-                rewrite bind_ret_l.
-
-                subst blah.
-                match goal with
-                | |- context[ITree.bind ?ma ?b] => remember b as blah
-                end.
-
-                rewrite interp_cfg_to_L3_ret.
-                rewrite tau_eutt.
-                rewrite bind_ret_l, translate_ret.
-                repeat rewrite translate_ret, interp_cfg_to_L3_ret.
-                rewrite translate_ret, bind_ret_l.
-
-                subst blah.
-                match goal with
-                | |- context[ITree.bind ?ma ?b] => remember b as blah
-                end.
-
-                repeat rewrite interp_cfg_to_L3_bind.
-                setoid_rewrite translate_ret.
-                rewrite interp_cfg_to_L3_ret.
-                rewrite bind_ret_l.
-                repeat rewrite interp_cfg_to_L3_bind.
-                repeat rewrite bind_bind.
-                rewrite translate_bind.
-                rewrite bind_bind.
-
-                epose proof (@denote_exp_nexp _ _ _ _ _ _ _ _ _ _ Hnexp_src).
-                Check eutt_clo_bind.
-                eapply eutt_clo_bind.
-
-                rewrite interp_intrinsics_vis.
-
-                destruct id eqn:Hid.
-                --- (* Name *)
-
-
-                  setoid_rewrite interp_interp.
-
-                --- (* Local id *)
-                admit.
-              ** (* Local id *)
-                admit.
-        -- (* exceptions *) admit.
-    + (* Need to handle exceptions *)
       admit.
-     *)
-    (* Focus 3. *)
-    (* cbn. *)
-    (* rewrite bind_ret_l. *)
-    (* destruct (nth_error σ v0) eqn:Herr'. *)
-    (* destruct d. *)
+  Admitted.
 
-    (* Focus 3. *)
+End GenIR.
 
-    (* (* Lookup failure *) *)
-    (* Focus 2. cbn. *)
-    (* unfold interp_Mem. *)
-    (* setoid_rewrite interp_state_bind. *)
-    (* unfold Exception.throw. *)
-    (* rewrite interp_state_vis. cbn. *)
-    (* unfold MDSHCOLOnFloat64.pure_state. *)
-    (* rewrite bind_vis. rewrite bind_vis. *)
-    (* unfold resum. unfold ReSum_inl. *)
-    (* unfold resum. unfold ReSum_id. *)
-    (* unfold id_. unfold inl_. *)
+Section LLVMGen.
+  
+  (** YZ TODO
+      This is initialized over the empty memory. That is incorrect. Run it over the initialze memory, and add the top level statement about compile
+     global_extern == false?
+   *)
+  Lemma LLVMGen_correct: forall R,
+    forall (* Compiler bits *) (s1 s2: IRState)
+      (* Helix bits *)    (i o: Int64.int) (globals: list (string*DSHType)) (globals_extern: bool) (fshcol: DSHOperator) (funname: string) (σ: evalContext)
+      (* Vellvm bits *)   tle,
+      LLVMGen i o globals false fshcol funname s1 ≡ inr (s2, tle) -> 
+      eutt (* (bisim_final σ) *) R
+           (translate_E_helix_mcfg
+                      (interp_Mem (denoteDSHOperator σ fshcol) memory_empty))
+           (semantics_llvm tle).
+  Proof.
+    (* intros p data pll H. *)
+    (*   unfold compile_w_main, compile in H. *)
+    (*   destruct p as [i o name globals op]. *)
+    (*   destruct (initIRGlobals data globals) as [? | [data' ginit]] eqn:EQGlob; [inv H |]. *)
+    (*   simpl in H. *)
+    (*   destruct (ErrorWithState.evalErrS (LLVMGen i o globals false op name) newState) eqn: EQEVALERR; [inv H | inv H]. *)
+    (*   unfold semantics_llvm. *)
+    (*   unfold semantics_llvm_mcfg. *)
+    (*   unfold lift_sem_to_mcfg. *)
+    (*   match goal with *)
+    (*     |- context[match ?p with | _ => _ end] => destruct p eqn:EQ *)
+    (*   end. { *)
+    (*     unfold ErrorWithState.evalErrS in EQEVALERR. *)
+    (*     destruct (LLVMGen i o globals false op name newState) eqn:EQGEN; inv EQEVALERR. *)
+  Admitted.
 
-    (* rewrite translate_vis. *)
-    (* unfold resum. unfold inr_. *)
-    (* Check VisF. *)
-    (* simpl. *)
-    (* unfold interp_state. unfold interp. *)
-    (* interp. *)
-    (* unfold Exception.Throw. cb *)
+End LLVMGen.
 
-    (* inversion H3. cbn. *)
-    (* simpl. *)
-    (* cbn. *)
-
-    (* subst i. *)
-    (* unfold interp_Mem; cbn. *)
-    (* destruct src, dst. *)
-    (* simpl in HCompile. *)
-    (* repeat break_match_hyp; try inl_inr. *)
-    (* inv Heqs; inv HCompile. *)
-    (* unfold denotePexp, evalPexp, lift_Serr. *)
-    (* subst. *)
-    (* unfold interp_Mem. (* cbn *) *)
-    (* (* match goal with *) *)
-    (* (* | |- context[add_comment _ ?ss] => generalize ss; intros ls *) *)
-    (* (* end. *) *)
-    (* (* match goal with *) *)
-    (* (* | |- context[add_comment _ ?ss] => generalize ss; intros ls1 *) *)
-    (* (* end. *) *)
-
-    (* (* subst. eutt_hide_right. *) *)
-    (* (* cbn. *) *)
-    (* (* unfold interp_Mem. *) *)
-    (* (* rewrite interp_state_bind. *) *)
-    (* (* unfold denotePexp, evalPexp. *) *)
-    (* (* cbn. *) *)
-    (* (* repeat setoid_rewrite interp_state_bind. *) *)
-    (* (* rewrite denote_bks_singleton. *) *)
-    (* (* destruct src, dst. *) *)
-    (* (* simpl in HCompile. *) *)
-    (* (* repeat break_match_hyp; try inl_inr. *) *)
-    (* (* inv Heqs; inv HCompile. *) *)
-    (* (* match goal with *) *)
-    (* (* | |- context[add_comment _ ?ss] => generalize ss; intros ls *) *)
-    (* (* end. *) *)
-    (* (* unfold interp_Mem. *) *)
-    (* (* simpl denoteDSHOperator. *) *)
-    (* (* rewrite interp_state_bind, translate_bind. *) *)
-    (* (* match goal with *) *)
-    (* (*   |- eutt _ ?t _ => remember t *) *)
-    (* (* end. *) *)
-
-    (* (* Need a lemma to invert Heqs2. *)
-    (*    Should allow us to know that the list of blocks is a singleton in this case. *)
-    (*    Need then probably a lemma to reduce proofs about `D.denote_bks [x]` to something like the denotation of x, *)
-    (*    avoiding having to worry about iter. *)
-    (*  *) *)
-    (* (* cbn; rewrite interp_cfg_to_L3_bind, interp_cfg_to_L3_ret, bind_ret_l. *) *)
-
-    (* repeat match goal with *)
-    (* | |- context [ String ?x ?y ] => remember (String x y) *)
-    (* end. *)
-
-    (* make_append_str in H6. *)
-    admit.
-  - (*
-      Map case.
-      Need some reasoning about
-      - denotePexp
-      - nat_eq_or_cerr
-      - genIMapBody
-      -
-     *)
-    simpl genIR in HCompile.
-
-    (* repeat rewrite string_cons_app in HCompile. *)
-
-    repeat break_match_hyp; try inl_inr.
-    repeat inv_sum.
-    cbn.
-    (* Need to solve the issue with the display of strings, it's just absurd *)
-    eutt_hide_right.
-    unfold interp_Mem.
-    rewrite interp_state_bind.
-    admit.
-
-  - admit.
-
-  - admit.
-
-  - admit.
-
-  - eutt_hide_right.
-    cbn. unfold interp_Mem.
-
-    (*
-    Check interp_state_bind.
-    Check interp_bind.
-
-interp_state_bind
-     : ∀ (f : ∀ T : Type, ?E T → ?S → itree ?F (?S * T)) (t : itree ?E ?A) (k : ?A → itree ?E ?B) (s : ?S),
-         interp_state f (ITree.bind t k) s
-         ≅ ITree.bind (interp_state f t s) (λ st0 : ?S * ?A, interp_state f (k (snd st0)) (fst st0))
-
-interp_bind
-     : ∀ (f : ∀ T : Type, ?E T → itree ?F T) (t : itree ?E ?R) (k : ?R → itree ?E ?S),
-         interp f (ITree.bind t k) ≅ ITree.bind (interp f t) (λ r : ?R, interp f (k r))
-
-    rewrite interp_state_bind.
-    rewrite interp_iter.
-*)
-    admit.
-
-  - eutt_hide_right.
-    cbn.
-    unfold interp_Mem.
-    rewrite interp_state_bind.
-    (* rewrite bind_trigger.
-
-    Locate ITree.bind.
-    rewrite *)
-    admit.
-  - admit.
-
-  - admit.
-
-  - (* Sequence case.
-
-     *)
-
-    cbn in HCompile.
-    break_match_hyp; try inv_sum.
-    break_match_hyp; try inv_sum.
-    destruct p, s.
-    break_match_hyp; try inv_sum.
-    destruct p, s; try inv_sum.
-    eapply IHop1 with (env := env) (σ := σ) in Heqs1; eauto.
-    eapply IHop2 with (env := env) (σ := σ) in Heqs0; eauto.
-    clear IHop2 IHop1.
-    eutt_hide_right.
-    cbn; unfold interp_Mem in *.
-    rewrite interp_state_bind.
-
-    rewrite translate_bind.
-    (* Opaque D.denote_bks. *)
-
-    (* Set Nested Proofs Allowed. *)
-
-    (* Lemma add_comment_app: forall bs1 bs2 s, *)
-    (*     add_comment (bs1 ++ bs2)%list s ≡ (add_comment bs1 s ++ add_comment bs2 s)%list. *)
-    (* Proof. *)
-    (*   induction bs1 as [| b bs1 IH]; cbn; auto; intros bs2 s. *)
-    (*   f_equal. rewrite IH; auto. *)
-
-    (*   subst i0. *)
-    (*   eutt_hide_left. *)
-    (*   cbn. rewrite bind_ret_l. *)
-
-
-(* Definition respectful_eutt {E F : Type -> Type} *)
-(*   : (itree E ~> itree F) -> (itree E ~> itree F) -> Prop *)
-(*   := i_respectful (fun _ => eutt eq) (fun _ => eutt eq). *)
-
-
-(* Instance eutt_translate {E F R} *)
-(*   : @Proper (IFun E F -> (itree E ~> itree F)) *)
-(*             (eq2 ==> eutt RR ==> eutt RR) *)
-(*             translate. *)
-(* Proof. *)
-(*   repeat red. *)
-(*   intros until T. *)
-(*   ginit. gcofix CIH. intros. *)
-(*   rewrite !unfold_translate. punfold H1. red in H1. *)
-(*   induction H1; intros; subst; simpl. *)
-(*   - gstep. econstructor. eauto. *)
-(*   - gstep. econstructor. pclearbot. eauto with paco. *)
-(*   - gstep. rewrite H. econstructor. pclearbot. red. eauto 7 with paco. *)
-(*   - rewrite tau_euttge, unfold_translate. eauto. *)
-(*   - rewrite tau_euttge, unfold_translate. eauto. *)
-(* Qed. *)
-
-(* Instance eutt_translate' {E F : Type -> Type} {R : Type} (f : E ~> F) : *)
-(*   Proper (eutt eq ==> eutt eq) *)
-(*          (@translate E F f R). *)
-(* Proof. *)
-(*   repeat red. *)
-(*   apply eutt_translate. *)
-(*   reflexivity. *)
-(* Qed. *)
-
-(*     rewrite Heqs1. *)
-(* eutt_translate' *)
-
-Admitted.
+(**
+   Initialization of the memory
+ **)
 
 Definition llvm_empty_memory_state_partial: LLVM_memory_state_cfg
   := (M.empty_memory_stack, ([], [])).
-
 
 (* This code attempts to mimic global variable initialization from
    [Vellvm.Toplevel] and heavily depends on internal memory
@@ -3222,19 +2333,6 @@ Admitted.
     just compare return value of [main] function in LLVM with
     evaulation results of DSHCOL.
  *)
-Definition bisim_final: Type_R_full :=
-  fun σ '(_, h_result) '(_,(_,(_,llvm_result))) =>
-    match llvm_result with
-    | UVALUE_Array arr => @List.Forall2 _ _
-                                       (fun ve de =>
-                                          match de with
-                                          | UVALUE_Double d =>
-                                            Floats.Float.cmp Integers.Ceq d ve
-                                          | _ => False
-                                          end)
-                                       h_result arr
-    | _ => False
-    end.
 
 Lemma bisim_partial_memory_subrelation: forall σ helix_state llvm_state,
     let '(mem_helix, _) := helix_state in
@@ -3248,18 +2346,18 @@ Proof.
   auto.
 Qed.
 
-Lemma bisim_full_partial_subrelation: forall σ helix_state llvm_state,
-    let '(mem_helix, v_helix) := helix_state in
-    let '(m, ((ρ,_), (g, v))) := llvm_state in
-    bisim_full σ helix_state llvm_state -> bisim_partial σ (mem_helix, tt) (mk_LLVM_sub_state_partial_from_mem (inr v) (m, (ρ, g))).
-Proof.
-  intros σ helix_state llvm_state.
-  repeat break_let.
-  subst.
-  intros H.
-  unfold mk_LLVM_sub_state_partial_from_mem.
-  auto.
-Qed.
+(* Lemma bisim_full_partial_subrelation: forall σ helix_state llvm_state, *)
+(*     let '(mem_helix, v_helix) := helix_state in *)
+(*     let '(m, ((ρ,_), (g, v))) := llvm_state in *)
+(*     bisim_full σ helix_state llvm_state -> bisim_partial σ (mem_helix, tt) (mk_LLVM_sub_state_partial_from_mem (inr v) (m, (ρ, g))). *)
+(* Proof. *)
+(*   intros σ helix_state llvm_state. *)
+(*   repeat break_let. *)
+(*   subst. *)
+(*   intros H. *)
+(*   unfold mk_LLVM_sub_state_partial_from_mem. *)
+(*   auto. *)
+(* Qed. *)
 
 (* Top-level compiler correctness lemma  *)
 Theorem compiler_correct:
